The *partial derivative* of $f(x,y)$, with respect to $x$ is the function $f_x(x,y)=\frac{\partial}{\partial x}f(x,y)$ obtained by differentiating $f$ with respect to $x$, treating $y$ as a constant

The *partial derivative* of $f(x,y)$, with respect to $y$ is the function $f_x(x,y)=\frac{\partial}{\partial y}f(x,y)$ obtained by differentiating $f$ with respect to $y$, treating $x$ as a constant

**No More Prime Notation!!! Hitler is dead**
- Use $f_x(x,y)$ or $f_y(x,y)$

## Higher order derivatives

- $(f_c)_c=\frac{\partial}{\partial x}(\frac{1})$ 

## Examples

1. Find the partial derivatives $f(x,y)=3x^2-2y+xy$
	- $f_x(x,y)=\frac{\partial f}{\partial x}(x,y)=\frac{\partial}{\partial x}(3x^2-2y+xy)=6x+y$
	- $f_y(x,y)=\frac{\partial f}{\partial y}=\frac{\partial}{\partial y}(3x^2-2y+xy)=-2+x$ 
2. $f(x,y)=e^{x+y^2}+ln(\frac{x}{x^2+y})=e^xe^{y^2}+ln(x)-ln(x^2+y)$ 
	- $f_x(x,y)=e^{x+y^2}+\frac{1}{x}-\frac{2x}{x^2+y}$
	- $f_y(x,y)=2ye^{x+y^2}-\frac{1}{x^2+y}$
3. $f(x,y,z)=3x^2z-e^y\sqrt{z}+\sqrt{x^2+y^2}$
	- $f_x(x,y,z)=6xz-\frac{x}{\sqrt{x^2+y^2}}$
	- $f_y(x,y,z)=e^y\sqrt{z}-\frac{y}{\sqrt{x^2+y^2}}$
	- $f_z(x,y,z)=3x^2-\frac{e^y}{2\sqrt{z}}$ 

