The gradient of a function $f(x,y)=\frac{\partial f}{\partial x}\hat{i}+\frac{\partial f}{\partial y}\hat{j}$

So if we have a (gradient) vector in the form
- $P(x,y)\hat{i}+Q(x,y)\hat{j}$
- We need
	- $P(x,y)=\frac{\partial f}{\partial x}(x,y)=f_x(x,y)$
	- $Q(x,y)=\frac{\partial f}{\partial y}(x,y)=f_y(x,y)$

Now when integrating $\frac{\partial f}{\partial x}$ with respect to $x$, remember that $y$ is a constant 

Recall the definition of a partition from calc 1.
- Definition: a partition of a closed interval $[a,b]$ is a finite subset of $[a,b]$ that contains the points $a$ and $b$
- When we say $\{x_0,x_1,\dots,x_n\}$ is a partition of $[a,b]$, we imply that $a=x_0<x_1<\dots<x_n=b$
- For example, the sets $P_1=\{0,1\}$, $P_2=\{0,\frac{1}{2},1\}$, $P_3=\{0,\frac{1}{10},\frac{1}{3},\frac{1}{2},,\frac{2}{3},\frac{7}{8},1\}$ are partitions of the interval $[0,1]$
- If $P=\{x_0,x_1,\dots,x_n\}$ is a partition of $[a,b]$, then $P$ breaks the interval into sub-intervals:
	- $[x_0,x_1],[x_1,x_2],[x_2,x_3],\dots[x_{n-1},x_n]$ lengths $\Delta x_1, \Delta x_2, \Delta x_3,\dots,\Delta x_n$.
- The lengths of these sub-intervals may or may not be equal

## Example

1. $xy^2\hat{i}+x^2y\hat{j}$
	- $\int (xy^2)dx=\frac{1}{2}x^2y^2+\phi (y)$
	- Set $f(x,y)=\frac{1}{2}x^2y^2+\phi(y)$ 
		- $f_y(x,y)=x^2y+\phi '(y)$
		- Want $f_y(x,y)=x^2+y$:
			- $x^2y+\phi '(y)=x^2y\implies \phi '(y)=0\implies \phi (y)=C$
	- Thus $f(x,y)=\frac{1}{2}x^2y^2+C$
	- Note: Sometimes the given vector could not be the gradient of a function. Can you think of a quick way to determine if a vector is a gradient? no
		- If $P(x,y)\hat{i}+Q(x,y)\hat{j}=\nabla f\implies P_y=Q_x=f_{xy}=f_{yx}$
2. $(y^2+x)\hat{i}+(x^2+y)\hat{j}$
	- $P_y=3y^2\ne Q_x=2x$
3. $(e^x+2xy)\hat{i}+(x^2+sin\ y)\hat{j}$
	- $P_y=Q_x=2x$
	- $\int Pdx=\int (e^x+2xy)dx=e^x+x^2y+\phi (y)$
	- Set $f(x,y)e^x+x^2y+\phi (y)$
		- $f_y=x^2+\phi '(y)$, $Q=x^2+sin(y)$
			- $\implies $\phi (y)=-cos(y)+C$
	- Thus, $f(x,y)=e^x+x^2y-cos(y)+C$
4. $(y^2+x)\hat{i}+(x^2+y^2)\hat{j}=P\hat{i}+Q\hat{j}$
	- $P_y=3y^2\ne Q_x=2x$
	- Thus the example cannot be a gradient
5. $(1+e^y)\hat{i}+(xe^y+y^2)\hat{j}=P\hat{i}+Q\hat{j}$
	-  $P_y=e^4=Q_x$
	- I will integrate Q with respect to y this time
	- $\int Q(x,y)dy=\int (xe^y+y^2)dy=xe^y+\frac{y^3}{3}+\phi(x)$
	- Let $f(x,y)=xe^y+\frac{1}{3}y^3+\phi(x)$
		- $f_x=e^y+0+\phi'(x)$, $P=1+ e^y$
		- $f_x=P\implies e^y+\phi'(x)=1+e^y$
		- $\phi'(x)=1$
		- $\phi(x)=x+C$
	- Now, $f(x,y)=xe^y+\frac{1}{3}y^3+x+C$
	- 