$$\nabla=\frac{\partial}{\partial x}\hat{i}+\frac{\partial}{\partial y}\hat{j}+\frac{\partial}{\partial z}\hat{k}$$
- So we are familiar with $\nabla$ from our work with gradients but how does this work with vector fields?
	- If $f(x,y,z)$ is a scalar field $\nabla f(x,y,z)=(\frac{\partial}{\partial x},\frac{\partial}{\partial y},\frac{\partial}{\partial z})f(x,y,z)=(\frac{\partial f}{\partial x},\frac{\partial f}{\partial y},\frac{\partial f}{\partial z})$
	- How does this work with $\overrightarrow{v}(x,y,z)=(v_1(x,y,z),v_2(x,y,z),v_3(x,y,z))$ 
- The divergence of $\overrightarrow{v}$ is
	- $div\ \overrightarrow{v}=\nabla \overrightarrow v=(\frac{\partial v_1}{\partial x},\frac{\partial v_2}{\partial y},\frac{\partial v_3}{\partial z})=\frac{\partial v_1}{\partial x}+ \frac{\partial v_2}{\partial y}+ \frac{\partial v_3}{\partial z}$
- The curl of $\overrightarrow{v}$ is 
	- $curl\ \overrightarrow{v}=\nabla \times \overrightarrow{v}=\hat{i}(\frac{\partial v_3}{\partial y}-\frac{\partial v_2}{\partial z})-\hat{j}(\frac{\partial v_3}{\partial x}-\frac{\partial v_1}{\partial z})+\hat{k}(\frac{\partial v_2}{\partial x}-\frac{\partial v_1}{\partial y})$
	- curl of a gradient is 0
- The divergence of a curl is zero

## Examples

1. Calculate $\nabla\cdot\overrightarrow{v}$ and $\nabla\times\overrightarrow{v}$ given:
	- $\overrightarrow{v}(x,y)=\frac{1}{x^2+y^2}\hat{i}+\frac{1}{x^2+y^2}\hat{j}$
	- $div(\overrightarrow{v})=\frac{\partial }{\partial x}(x^2+y^2)^{-1}+\frac{\partial }{\partial y}(x^2+y^2)^{-1}=\frac{-2x-2y}{(x^2+y^2)^{-2}}$
	- $curl(\overrightarrow{v})=\nabla\times\overrightarrow{v}=\hat{i}(0-0)-\hat{j}(0-0)+\hat{k}(\frac{-2x}{(x^2+y^2)^2}+\frac{2y}{(x^2+y^2)^2})=\frac{2y-2x}{(x^2+y^2)^2}\hat{k}$
		- $curl$ will be solely in the $\hat{k}$ direction if $\overrightarrow{v}$ doesn't vary with $z$
2. Calculate $\nabla\cdot\overrightarrow{v}$ and $\nabla\times\overrightarrow{v}$ given:
	- $\overrightarrow{v}(x,y,z)=2yz\hat{i}+4xz\hat{j}+3xy\hat{k}$
	- $div(\overrightarrow{v})=0$
	- $curl(\overrightarrow{v})=\nabla\times\overrightarrow{v}=\hat{i}(3x-4x)-\hat{j}(3y-3y)+\hat{k}(4z-3z)=(-x,0,z)$
